fix: refactor ToInt.OfNat (#9005)
This PR changes the definition of `Lean.Grind.ToInt.OfNat`, introducing
a `wrap` on the right-hand-side.

src/Init/Grind/Ring/ToInt.lean
@@ -13,21 +13,15 @@ namespace Lean.Grind
 
 /-- A `ToInt` instance on a semiring preserves powers if it preserves numerals and multiplication. -/
 def ToInt.pow_of_semiring [Semiring α] [ToInt α I] [ToInt.OfNat α I] [ToInt.Mul α I]
-    (h₁ : I.isFinite) (h₂ : 1 ∈ I) : ToInt.Pow α I where
+    (h₁ : I.isFinite) : ToInt.Pow α I where
   toInt_pow x n := by
     induction n with
     | zero =>
-      rw [Semiring.pow_zero]
-      rw [ToInt.OfNat.toInt_ofNat _ h₂]
-      rw [Int.pow_zero]
-      rw [(I.wrap_eq_self_iff (IntInterval.nonEmpty_of_mem h₂) _).mpr h₂]
+      rw [Semiring.pow_zero, ToInt.OfNat.toInt_ofNat, Int.pow_zero]
       rfl
     | succ n ih =>
-      rw [Semiring.pow_succ]
-      rw [ToInt.Mul.toInt_mul]
+      rw [Semiring.pow_succ, ToInt.Mul.toInt_mul]
       conv => lhs; rw [← ToInt.wrap_toInt I x]
-      rw [ih]
-      rw [← I.wrap_mul h₁]
-      rw [Int.pow_succ]
+      rw [ih, ← I.wrap_mul h₁, Int.pow_succ]
 
 end Lean.Grind
